Fix einst

theories/Inst.v
@@ -5,25 +5,29 @@ From LocalComp.autosubst Require Import AST SubstNotations RAsimpl AST_rasimpl.
 From LocalComp Require Import Util BasicAST Env.
 Import ListNotations.
 
-(**
+Definition eget (ξ : eargs) M x :=
+  let default := assm M x in (* Could also be a dummy *)
+  match nth_error ξ M with
+  | Some σ =>
+    match nth_error σ x with
+    | Some t => t
+    | None => default
+    end
+  | None => default
+  end.
 
-  The argument [t] of [einst ξ t] is expected to be closed.
-  This is the reason why we use a dummy value for variables, this way we don't
-  need to worry about the function being partial.
-  Thanks to this, we also don't need to worry about lifting [ξ] when going under
-  binders.
+Definition ren_eargs ρ (ξ : eargs) : eargs :=
+  map (map (ren_term ρ)) ξ.
 
-**)
-
-Definition dummy := Sort 0.
+Notation lift_eargs ξ := (ren_eargs S ξ).
 
 Fixpoint einst (ξ : eargs) (t : term) :=
   match t with
-  | var n => dummy
+  | var n => var n
   | Sort i => Sort i
-  | Pi A B => Pi (einst ξ A) (einst ξ B)
-  | lam A t => lam (einst ξ A) (einst ξ t)
+  | Pi A B => Pi (einst ξ A) (einst (lift_eargs ξ) B)
+  | lam A t => lam (einst ξ A) (einst (lift_eargs ξ) t)
   | app u v => app (einst ξ u) (einst ξ v)
   | const c ξ' => const c (map (map (einst ξ)) ξ')
-  | assm M x => assm M x
+  | assm M x => eget ξ M x
   end.
